Add some stuff for propositional logic.

LogicBase.v
@@ -5,56 +5,23 @@ Class Language: Type := {
   expr: Type
 }.
 
-Class NormalLanguage {L: Language}: Type := {
+Class NormalLanguage (L: Language): Type := {
   FF: expr;
   imp: expr -> expr -> expr
 }.
 
 Definition context {L: Language}: Type := Ensemble expr.
 
+Definition empty_context {L: Language}: context := Empty_set _.
+
 Class ProofTheory (L: Language): Type := {
   provable: expr -> Prop;
-  derives: context -> expr -> Prop
+  derivable: context -> expr -> Prop;
+  provable_derivable: forall x, provable x <-> derivable empty_context x
 }.
 
-Definition consistent {L: Language} {nL: NormalLanguage} {Sigma: ProofTheory L}: context -> Prop :=
-  fun Gamma => ~ derives Gamma FF.
-
-Module AxiomaticProofTheory.
-
-Class ProofTheory (L: Language): Type := {
-  provable: expr -> Prop
-}.
-
-Definition multi_imp {L: Language} {nL: NormalLanguage}: list expr -> expr -> expr :=
-  fix f (xs: list expr) (y: expr): expr :=
-    match xs with
-    | nil => y
-    | x0 :: xs' => imp x0 (f xs' y)
-    end.
-
-Definition derives {L: Language} {nL: NormalLanguage} {Sigma: ProofTheory L}: context -> expr -> Prop :=
-  fun Gamma y =>
-    exists xs, Included expr (fun x => In x xs) Gamma /\ provable (multi_imp xs y).
-
-End AxiomaticProofTheory.
-
-Instance AxiomaticProofTheory_ProofTheory {L: Language} {nL: NormalLanguage} (Sigma: AxiomaticProofTheory.ProofTheory L): ProofTheory L :=
-  Build_ProofTheory L AxiomaticProofTheory.provable (AxiomaticProofTheory.derives).
-
-Module SequentCalculus.
-
-Class ProofTheory (L: Language): Type := {
-  derives: context -> expr -> Prop
-}.
-
-Definition provable {L: Language} {Sigma: ProofTheory L}: expr -> Prop :=
-  fun x => derives (Empty_set _) x.
-
-End SequentCalculus.
-
-Instance SequentCalculus {L: Language} (Sigma: SequentCalculus.ProofTheory L): ProofTheory L :=
-  Build_ProofTheory L SequentCalculus.provable SequentCalculus.derives.
+Definition consistent {L: Language} {nL: NormalLanguage L} {Gamma: ProofTheory L}: context -> Prop :=
+  fun Phi => ~ derivable Phi FF.
 
 Class Semantics (L: Language): Type := {
   model: Type;
@@ -62,15 +29,79 @@ Class Semantics (L: Language): Type := {
 }.
 
 Definition consequence {L: Language} {SM: Semantics L}: context -> expr -> Prop :=
-  fun Gamma y =>
-    forall m: model, (forall x, Gamma x -> satisfies m x) -> satisfies m y.
+  fun Phi y =>
+    forall m: model, (forall x, Phi x -> satisfies m x) -> satisfies m y.
 
 Definition valid {L: Language} {SM: Semantics L}: expr -> Prop :=
   fun x =>
     forall m: model, satisfies m x.
 
 Definition satisfiable {L: Language} {SM: Semantics L}: context -> Prop :=
-  fun Gamma =>
-    exists m: model, forall x: expr, Gamma x -> satisfies m x.
+  fun Phi =>
+    exists m: model, forall x: expr, Phi x -> satisfies m x.
 
-Definition sound {L: Language} (Sigma: ProofTheory L) (SM: Semantics L): 
+Definition sound {L: Language} (Gamma: ProofTheory L) (SM: Semantics L): Prop :=
+  forall x: expr, provable x -> valid x.
+
+Definition weakly_complete {L: Language} (Gamma: ProofTheory L) (SM: Semantics L): Prop :=
+  forall x: expr, valid x -> provable x.
+
+Definition strongly_complete {L: Language} (Gamma: ProofTheory L) (SM: Semantics L): Prop :=
+  forall (Phi: context) (x: expr), consequence Phi x -> derivable Phi x.
+
+
+Module AxiomaticProofTheory.
+
+Class ProofTheory (L: Language): Type := {
+  provable: expr -> Prop
+}.
+
+Definition multi_imp {L: Language} {nL: NormalLanguage L}: list expr -> expr -> expr :=
+  fix f (xs: list expr) (y: expr): expr :=
+    match xs with
+    | nil => y
+    | x0 :: xs' => imp x0 (f xs' y)
+    end.
+
+Definition derivable {L: Language} {nL: NormalLanguage L} {Gamma: ProofTheory L}: context -> expr -> Prop :=
+  fun Phi y =>
+    exists xs, Included expr (fun x => In x xs) Phi /\ provable (multi_imp xs y).
+
+Lemma provable_derivable {L: Language} {nL: NormalLanguage L} {Gamma: ProofTheory L}: forall x, provable x <-> derivable empty_context x.
+Proof.
+  intros.
+  split; intros.
+  + exists nil; split; auto.
+    hnf; intros.
+    inversion H0.
+  + destruct H as [xs [? ?]].
+    destruct xs; [auto |].
+    specialize (H e (or_introl eq_refl)).
+    inversion H.
+Qed.
+
+End AxiomaticProofTheory.
+
+Instance AxiomaticProofTheory_ProofTheory {L: Language} {nL: NormalLanguage L} (Gamma: AxiomaticProofTheory.ProofTheory L): ProofTheory L :=
+  Build_ProofTheory L AxiomaticProofTheory.provable AxiomaticProofTheory.derivable AxiomaticProofTheory.provable_derivable.
+
+Module SequentCalculus.
+
+Class ProofTheory (L: Language): Type := {
+  derivable: context -> expr -> Prop
+}.
+
+Definition provable {L: Language} {Gamma: ProofTheory L}: expr -> Prop :=
+  fun x => derivable (Empty_set _) x.
+
+End SequentCalculus.
+
+Instance SequentCalculus {L: Language} (Gamma: SequentCalculus.ProofTheory L): ProofTheory L :=
+  Build_ProofTheory L SequentCalculus.provable SequentCalculus.derivable (fun x => iff_refl _).
+
+Notation "m  |=  x" := (satisfies m x) (at level 60, no associativity) : logic_base.
+Notation "|==  x" := (valid x) (at level 61, no associativity) : logic_base.
+Notation "Phi  |==  x" := (consequence Phi x) (at level 60, no associativity) : logic_base.
+Notation "|--  x" := (provable x) (at level 61, no associativity) : logic_base.
+Notation "Phi  |--  x" := (derivable Phi x) (at level 60, no associativity) : logic_base.
+
