PropositionalLogic/ClassicalPropositionalLogic.v
@@ -1,0 +1,28 @@
+Require Import Logic.LogicBase.
+Require Import Logic.PropositionalLogic.Syntax.
+
+Local Open Scope PropositionalLogic.
+
+Section ClassicalPropositionalLogic.
+
+Context {Var: Type}.
+
+Definition reduce: expr Var -> expr Var -> Prop :=
+  syntax_reduce
+   (fun x y =>
+      ImpNegAsPrime.atomic_reduce x y \/
+      ReduceIff.atomic_reduce x y \/
+      ReduceTrueFalse.atomic_reduce x y).
+
+Inductive provable: expr Var -> Prop :=
+| syntactic_reduction_rule: forall x y, reduce x y -> provable x -> provable y
+| modus_ponens: forall x y, provable (x --> y) -> provable x -> provable y
+| axiom1: forall x y, provable (x --> (y --> x))
+| axiom2: forall x y z, provable ((x --> y --> z) --> (x --> y) --> (x --> z))
+| axiom3: forall x y, provable ((~~ y --> x) --> (~~ y --> ~~ x) --> y).
+
+End ClassicalPropositionalLogic.
+
+Instance ClassicalPropositionLogic (Var: Type): ProofTheory (PropositionalLanguage Var) :=
+  AxiomaticProofTheory_ProofTheory
+   (AxiomaticProofTheory.Build_ProofTheory (PropositionalLanguage Var) provable).
