PropositionalLogic/Syntax.v
@@ -1,0 +1,75 @@
+Require Import Logic.LogicBase.
+
+Inductive expr {Var: Type}: Type :=
+  | andp : expr -> expr -> expr
+  | orp : expr -> expr -> expr
+  | imp : expr -> expr -> expr
+  | iffp : expr -> expr -> expr
+  | negp : expr -> expr
+  | truep : expr
+  | falsep : expr
+  | varp : Var -> expr.
+
+Implicit Arguments expr.
+
+Notation "x && y" := (andp x y) (at level 40, left associativity) : PropositionalLogic.
+Notation "x || y" := (orp x y) (at level 50, left associativity) : PropositionalLogic.
+Notation "x --> y" := (imp x y) (at level 55, right associativity) : PropositionalLogic.
+Notation "x <--> y" := (iffp x y) (at level 60, no associativity) : PropositionalLogic.
+Notation "~~ x" := (negp x) (at level 35) : PropositionalLogic.
+Notation "'FF'" := falsep : PropositionalLogic.
+Notation "'TT'" := truep : PropositionalLogic.
+
+Local Open Scope PropositionalLogic.
+
+Instance PropositionalLanguage (Var: Type): Language := Build_Language (expr Var).
+
+Instance nPropositionalLanguage (Var: Type): NormalLanguage (PropositionalLanguage Var) :=
+  Build_NormalLanguage (PropositionalLanguage Var) FF imp.
+
+Inductive syntax_reduce {Var: Type} {atomic_reduce: expr Var -> expr Var -> Prop}:  expr Var -> expr Var -> Prop :=
+| atomic_step: forall x y, atomic_reduce x y -> syntax_reduce x y
+| reduce_refl: forall x, syntax_reduce x x
+| reduce_trans: forall x y z, syntax_reduce x y -> syntax_reduce y z -> syntax_reduce x z
+| andp_congr: forall x1 x2 y1 y2, syntax_reduce x1 y1 -> syntax_reduce x2 y2 -> syntax_reduce (x1 && x2) (y1 && y2)
+| orp_congr: forall x1 x2 y1 y2, syntax_reduce x1 y1 -> syntax_reduce x2 y2 -> syntax_reduce (x1 || x2) (y1 || y2)
+| imp_congr: forall x1 x2 y1 y2, syntax_reduce x1 y1 -> syntax_reduce x2 y2 -> syntax_reduce (x1 --> x2) (y1 --> y2)
+| iffp_congr: forall x1 x2 y1 y2, syntax_reduce x1 y1 -> syntax_reduce x2 y2 -> syntax_reduce (x1 <--> x2) (y1 <--> y2)
+| negp_congr: forall x y, syntax_reduce x y -> syntax_reduce (~~ x) (~~ y)
+.
+
+Arguments syntax_reduce {Var} atomic_reduce _ _.
+
+Module ImpNegAsPrime.
+
+Inductive atomic_reduce {Var: Type}: expr Var -> expr Var -> Prop :=
+| andp_reduce: forall x y, atomic_reduce (x && y) (~~ (x --> ~~ y))
+| orp_reduce: forall x y, atomic_reduce (x || y) (~~ x --> y)
+.
+
+End ImpNegAsPrime.
+
+Module ImpAndOrAsPrime.
+
+Inductive atomic_reduce {Var: Type}: expr Var -> expr Var -> Prop :=
+| negp_reduce: forall x, atomic_reduce (~~ x) (x --> FF)
+.
+
+End ImpAndOrAsPrime.
+
+Module ReduceIff.
+
+Inductive atomic_reduce {Var: Type}: expr Var -> expr Var -> Prop :=
+| iff_reduce: forall x y, atomic_reduce (x <--> y) ((x --> y) && (y --> x)).
+
+End ReduceIff.
+
+Module ReduceTrueFalse.
+
+Inductive atomic_reduce {Var: Type}: expr Var -> expr Var -> Prop :=
+| falsep_reduce: atomic_reduce FF (~~ TT)
+| truep_reduce: forall x, atomic_reduce TT (x --> x).
+
+End ReduceTrueFalse.
+
+
