Makefile
@@ -2,6 +2,6 @@ COQC = coqc
 
 %.vo: %.v
 	@echo COQC $*.v
-	@$(COQC) -q -R "." -as IntuitionisticLogic $*.v
+	@$(COQC) -q -R "." -as Logic $*.v
 
-all: Wf.vo base.vo IPC.vo trivial.vo Kripke.vo enumerate.vo
+all: Wf.vo base.vo IPC.vo trivial.vo Kripke.vo enumerate.vo LogicBase.vo PropositionalLogic/Syntax.vo PropositionalLogic/ClassicalPropositionalLogic.vo
